add bn_get_num_bits

tests/bignum4096-test.c
@@ -11,7 +11,6 @@
 
 
 bool mod_exp_bytes_be_precompr2(
-  uint32_t nBits,
   uint8_t *nBytes,
   uint8_t *aBytes,
   uint32_t bBits,
@@ -25,7 +24,7 @@ bool mod_exp_bytes_be_precompr2(
   uint64_t *a = Hacl_Bignum4096_new_bn_from_bytes_be(512, aBytes);
   uint64_t *n = Hacl_Bignum4096_new_bn_from_bytes_be(512, nBytes);
   uint64_t *b = Hacl_Bignum4096_new_bn_from_bytes_be(bBytesLen, bBytes);
-  uint64_t *r2 = Hacl_Bignum4096_new_precompr2(nBits, 64, n);
+  uint64_t *r2 = Hacl_Bignum4096_new_precompr2(64, n);
 
   Hacl_Bignum4096_mod_exp_precompr2(n, a, bBits, b, r2, res);
   Hacl_Bignum4096_bn_to_bytes_be(res, resBytes);
@@ -35,7 +34,6 @@ bool mod_exp_bytes_be_precompr2(
 
 
 bool mod_exp_bytes_be(
-  uint32_t nBits,
   uint8_t *nBytes,
   uint8_t *aBytes,
   uint32_t bBits,
@@ -50,14 +48,13 @@ bool mod_exp_bytes_be(
   uint64_t *n = Hacl_Bignum4096_new_bn_from_bytes_be(512, nBytes);
   uint64_t *b = Hacl_Bignum4096_new_bn_from_bytes_be(bBytesLen, bBytes);
 
-  Hacl_Bignum4096_mod_exp(nBits, n, a, bBits, b, res);
+  Hacl_Bignum4096_mod_exp(n, a, bBits, b, res);
   Hacl_Bignum4096_bn_to_bytes_be(res, resBytes);
 
   return 1;
 }
 
 bool print_test_bytes_be_precompr2(
-  uint32_t nBits,
   uint8_t *nBytes,
   uint8_t *aBytes,
   uint32_t bBits,
@@ -66,7 +63,7 @@ bool print_test_bytes_be_precompr2(
 )
 {
   uint8_t resBytes[512U] = {0};
-  bool ok = mod_exp_bytes_be_precompr2(nBits, nBytes, aBytes, bBits, bBytes, resBytes);
+  bool ok = mod_exp_bytes_be_precompr2(nBytes, aBytes, bBits, bBytes, resBytes);
   printf("\n mod_exp_precompr2 for bytes Result: \n");
   ok = ok && compare_and_print(512U, resBytes, resBytes_expected);
 
@@ -75,7 +72,6 @@ bool print_test_bytes_be_precompr2(
 
 
 bool print_test_bytes_be(
-  uint32_t nBits,
   uint8_t *nBytes,
   uint8_t *aBytes,
   uint32_t bBits,
@@ -84,7 +80,7 @@ bool print_test_bytes_be(
 )
 {
   uint8_t resBytes[512U] = {0};
-  bool ok = mod_exp_bytes_be(nBits, nBytes, aBytes, bBits, bBytes, resBytes);
+  bool ok = mod_exp_bytes_be(nBytes, aBytes, bBits, bBytes, resBytes);
   printf("\n mod_exp for bytes Result: \n");
   ok = ok && compare_and_print(512U, resBytes, resBytes_expected);
 
@@ -93,7 +89,6 @@ bool print_test_bytes_be(
 
 
 bool print_test(
-  uint32_t nBits,
   uint64_t *n,
   uint64_t *a,
   uint32_t bBits,
@@ -102,7 +97,7 @@ bool print_test(
 )
 {
   uint64_t res[64U] = {0};
-  Hacl_Bignum4096_mod_exp(nBits, n, a, bBits, b, res);
+  Hacl_Bignum4096_mod_exp(n, a, bBits, b, res);
   printf("\n mod_exp Result: \n");
 
   bool ok = true;
@@ -121,15 +116,15 @@ int main() {
 
   bool ok = true;
   for (int i = 0; i < sizeof(vectors_be)/sizeof(bignum4096_bytes_be_test_vector); ++i) {
-    ok &= print_test_bytes_be_precompr2(vectors_be[i].nBits,vectors_be[i].nBytes, vectors_be[i].aBytes, vectors_be[i].bBits, vectors_be[i].bBytes, vectors_be[i].resBytes);
+    ok &= print_test_bytes_be_precompr2(vectors_be[i].nBytes, vectors_be[i].aBytes, vectors_be[i].bBits, vectors_be[i].bBytes, vectors_be[i].resBytes);
   }
 
   for (int i = 0; i < sizeof(vectors_be)/sizeof(bignum4096_bytes_be_test_vector); ++i) {
-    ok &= print_test_bytes_be(vectors_be[i].nBits,vectors_be[i].nBytes, vectors_be[i].aBytes, vectors_be[i].bBits, vectors_be[i].bBytes, vectors_be[i].resBytes);
+    ok &= print_test_bytes_be(vectors_be[i].nBytes, vectors_be[i].aBytes, vectors_be[i].bBits, vectors_be[i].bBytes, vectors_be[i].resBytes);
   }
 
   for (int i = 0; i < sizeof(vectors)/sizeof(bignum4096_test_vector); ++i) {
-    ok &= print_test(vectors_be[i].nBits,vectors[i].n, vectors[i].a, vectors[i].bBits, vectors[i].b, vectors[i].res);
+    ok &= print_test(vectors[i].n, vectors[i].a, vectors[i].bBits, vectors[i].b, vectors[i].res);
   }
 
   if (ok) return EXIT_SUCCESS;
