code/bignum/Hacl.Bignum.Exponentiation.fsti
@@ -58,41 +58,37 @@ val bn_mod_exp_mont_ladder_precompr2: nLen:_ -> bn_mod_exp_mont_ladder_precompr2
 
 // This function is *NOT* constant-time on the exponent b
 inline_for_extraction noextract
-let bn_mod_exp_st (nLen:size_t{0 < v nLen /\ 128 * v nLen <= max_size_t})
-  (nBits:size_t{0 < v nBits})
- =
+let bn_mod_exp_st (nLen:size_t{0 < v nLen /\ 128 * v nLen <= max_size_t}) =
     n:lbignum nLen
   -> a:lbignum nLen
   -> bBits:size_t{v bBits > 0}
   -> b:lbignum (blocks bBits 64ul)
   -> res:lbignum nLen ->
   Stack unit
-  (requires fun h ->
+  (requires fun h -> 1 < bn_v h n /\
     live h n /\ live h a /\ live h b /\ live h res /\
     disjoint res a /\ disjoint res b /\ disjoint res n /\ disjoint n a)
   (ensures  fun h0 _ h1 -> modifies (loc res) h0 h1 /\
-    as_seq h1 res == S.bn_mod_exp (v nLen) (v nBits) (as_seq h0 n) (as_seq h0 a) (v bBits) (as_seq h0 b))
+    as_seq h1 res == S.bn_mod_exp (v nLen) (as_seq h0 n) (as_seq h0 a) (v bBits) (as_seq h0 b))
 
 // This version is fully run-time.
-val bn_mod_exp: nLen:_ -> nBits:_ -> bn_mod_exp_st nLen nBits
+val bn_mod_exp: nLen:_ -> bn_mod_exp_st nLen
 
 
 // This function is constant-time on the exponent b
 inline_for_extraction noextract
-let bn_mod_exp_mont_ladder_st (nLen:size_t{0 < v nLen /\ 128 * v nLen <= max_size_t})
-  (nBits:size_t{0 < v nBits})
- =
+let bn_mod_exp_mont_ladder_st (nLen:size_t{0 < v nLen /\ 128 * v nLen <= max_size_t}) =
     n:lbignum nLen
   -> a:lbignum nLen
   -> bBits:size_t{v bBits > 0}
   -> b:lbignum (blocks bBits 64ul)
   -> res:lbignum nLen ->
   Stack unit
-  (requires fun h ->
+  (requires fun h -> 1 < bn_v h n /\
     live h n /\ live h a /\ live h b /\ live h res /\
     disjoint res a /\ disjoint res b /\ disjoint res n /\ disjoint n a)
   (ensures  fun h0 _ h1 -> modifies (loc res) h0 h1 /\
-    as_seq h1 res == S.bn_mod_exp_mont_ladder (v nLen) (v nBits) (as_seq h0 n) (as_seq h0 a) (v bBits) (as_seq h0 b))
+    as_seq h1 res == S.bn_mod_exp_mont_ladder (v nLen) (as_seq h0 n) (as_seq h0 a) (v bBits) (as_seq h0 b))
 
 // This version is fully run-time.
-val bn_mod_exp_mont_ladder: nLen:_ -> nBits:_ -> bn_mod_exp_mont_ladder_st nLen nBits
+val bn_mod_exp_mont_ladder: nLen:_ -> bn_mod_exp_mont_ladder_st nLen
