code/bignum/Hacl.Spec.Bignum.Base.fst
@@ -46,24 +46,24 @@ let subborrow_u64 cin x y =
 
 
 
-let mask_values (x:uint64) =
-  v x = v (zeros U64 SEC) \/ v x = v (ones U64 SEC)
+let mask_values (#t:inttype{unsigned t}) (x:uint_t t SEC) =
+  v x = v (zeros t SEC) \/ v x = v (ones t SEC)
 
 inline_for_extraction noextract
-val mask_select: mask:uint64 -> a:uint64 -> b:uint64 -> uint64
+val mask_select: #t:inttype{unsigned t} -> mask:uint_t t SEC -> a:uint_t t SEC -> b:uint_t t SEC -> uint_t t SEC
 let mask_select mask a b =
   (mask &. a) |. ((lognot mask) &. b)
 
-val mask_select_lemma: mask:uint64 -> a:uint64 -> b:uint64 -> Lemma
+val mask_select_lemma: #t:inttype{unsigned t} -> mask:uint_t t SEC -> a:uint_t t SEC -> b:uint_t t SEC -> Lemma
   (requires mask_values mask)
   (ensures  mask_select mask a b == (if v mask = 0 then b else a))
 
-let mask_select_lemma mask a b =
+let mask_select_lemma #t mask a b =
   if v mask = 0 then begin
     logand_lemma mask a;
     assert (v (mask &. a) = 0);
     lognot_lemma mask;
-    assert (v (lognot mask) = v (ones U64 SEC));
+    assert (v (lognot mask) = v (ones t SEC));
     logand_lemma (lognot mask) b;
     assert (v ((lognot mask) &. b) == v b);
     logor_lemma (mask &. a) ((lognot mask) &. b);
@@ -77,6 +77,26 @@ let mask_select_lemma mask a b =
     assert (v ((lognot mask) &. b) == 0);
     logor_zeros (mask &. a);
     assert (v (mask_select mask a b) == v a) end
+
+
+val mask_select_lemma1: mask:uint64 -> a:uint64 -> b:uint64 -> Lemma
+  (requires mask_values mask)
+  (ensures  b ^. (mask &. (a ^. b)) == (if v mask = 0 then b else a))
+
+let mask_select_lemma1 mask a b =
+  let t1 = mask &. (a ^. b) in
+  let t2 = b ^. t1 in
+  logand_lemma mask (a ^.b);
+  if v mask = 0 then begin
+    assert (v t1 == 0);
+    logxor_lemma b t1;
+    assert (v t2 = v b);
+    () end
+  else begin
+    assert (v t1 == v (a ^. b));
+    logxor_lemma b a;
+    assert (v t2 = v a);
+    () end
 
 
 val lseq_mask_select_lemma: #len:size_nat ->a:lseq uint64 len -> b:lseq uint64 len -> mask:uint64 -> Lemma
