code/bignum/Hacl.Spec.Bignum.Lib.fst
@@ -9,6 +9,8 @@ open Hacl.Spec.Bignum.Definitions
 
 module BSeq = Lib.ByteSequence
 module Loops = Lib.LoopCombinators
+module BB = Hacl.Spec.Bignum.Base
+
 
 #set-options "--z3rlimit 50 --fuel 0 --ifuel 0"
 
@@ -16,23 +18,35 @@ module Loops = Lib.LoopCombinators
 ///  Get and set i-th bit of a bignum
 ///
 
+val limb_get_ith_bit: a:uint64 -> i:nat{i < 64} -> uint64
+let limb_get_ith_bit a i = (a >>. size i) &. u64 1
+
+val limb_get_ith_bit_lemma: a:uint64 -> i:nat{i < 64} ->
+  Lemma (v (limb_get_ith_bit a i) == v a / pow2 i % 2)
+
+let limb_get_ith_bit_lemma a i =
+  let tmp1 = a >>. size i in
+  let tmp2 = tmp1 &. u64 1 in
+  mod_mask_lemma tmp1 1ul;
+  assert (v (mod_mask #U64 #SEC 1ul) == v (u64 1));
+  assert (v tmp2 == v a / pow2 i % 2)
+
 val bn_get_ith_bit: #len:size_nat -> b:lbignum len -> i:size_nat{i / 64 < len} -> uint64
 let bn_get_ith_bit #len input ind =
   let i = ind / 64 in
   let j = ind % 64 in
-  (input.[i] >>. size j) &. u64 1
+  limb_get_ith_bit input.[i] j
+
 
 #push-options "--z3rlimit 100"
 val bn_get_ith_bit_lemma: #len:size_nat -> b:lbignum len -> i:size_nat{i / 64 < len} ->
   Lemma (v (bn_get_ith_bit b i) == (bn_v b / pow2 i % 2))
+
 let bn_get_ith_bit_lemma #len b ind =
   let i = ind / 64 in
   let j = ind % 64 in
-  let tmp1 = b.[i] >>. size j in
-  let tmp2 = tmp1 &. u64 1 in
-  mod_mask_lemma tmp1 1ul;
-  assert (v (mod_mask #U64 #SEC 1ul) == v (u64 1));
-  assert (v tmp2 == v b.[i] / pow2 j % 2);
+  let res = limb_get_ith_bit b.[i] j in
+  limb_get_ith_bit_lemma b.[i] j;
 
   calc (==) {
     v b.[i] / pow2 j % 2;
@@ -40,17 +54,19 @@ let bn_get_ith_bit_lemma #len b ind =
     (bn_v b / pow2 (64 * i) % pow2 64) / pow2 j % 2;
     (==) { Math.Lemmas.pow2_modulo_division_lemma_1 (bn_v b / pow2 (64 * i)) j 64 }
     (bn_v b / pow2 (64 * i) / pow2 j) % pow2 (64 - j) % 2;
-    (==) { Math.Lemmas.pow2_modulo_modulo_lemma_1 (bn_v b / pow2 (64 * i) / pow2 j) 1 (64 - j) }
-    (bn_v b / pow2 (64 * i) / pow2 j) % 2;
     (==) { Math.Lemmas.division_multiplication_lemma (bn_v b) (pow2 (64 * i)) (pow2 j) }
-    (bn_v b / (pow2 (64 * i) * pow2 j)) % 2;
+    (bn_v b / (pow2 (64 * i) * pow2 j)) % pow2 (64 - j) % 2;
     (==) { Math.Lemmas.pow2_plus (64 * i) j }
-    bn_v b / pow2 (64 * i + j) % 2;
+    (bn_v b / pow2 (64 * i + j)) % pow2 (64 - j) % 2;
     (==) { Math.Lemmas.euclidean_div_axiom ind 64 }
-    bn_v b / pow2 ind % 2;
-  };
-  assert (v tmp2 == bn_v b / pow2 ind % 2)
+    (bn_v b / pow2 ind) % pow2 (64 - j) % 2;
+    (==) { assert_norm (pow2 1 = 2);
+           Math.Lemmas.pow2_modulo_modulo_lemma_1 (bn_v b / pow2 ind) 1 (64 - j) }
+    (bn_v b / pow2 ind) % 2;
+    };
+  assert (v res == bn_v b / pow2 ind % 2)
 #pop-options
+
 
 val bn_set_ith_bit: #len:size_nat -> b:lbignum len -> i:size_nat{i / 64 < len} -> lbignum len
 let bn_set_ith_bit #len input ind =
@@ -63,6 +79,7 @@ let bn_set_ith_bit #len input ind =
 val bn_set_ith_bit_lemma_aux: a:nat -> b:nat -> c:nat -> d:nat -> Lemma
   (requires a + b * pow2 c < pow2 (c + d) /\ a < pow2 c)
   (ensures  b < pow2 d)
+
 let bn_set_ith_bit_lemma_aux a b c d =
   Math.Lemmas.lemma_div_lt_nat (a + b * pow2 c) (c + d) c;
   assert ((a + b * pow2 c) / pow2 c < pow2 d);
@@ -105,6 +122,7 @@ let bn_lt_pow2_index_lemma #len b ind =
 val bn_set_ith_bit_lemma: #len:size_nat -> b:lbignum len -> i:size_nat{i / 64 < len} -> Lemma
   (requires bn_v b < pow2 i)
   (ensures  bn_v (bn_set_ith_bit b i) == bn_v b + pow2 i)
+
 let bn_set_ith_bit_lemma #len input ind =
   let i = ind / 64 in
   let j = ind % 64 in
@@ -149,6 +167,7 @@ val bn_div_pow2: #len:size_nat -> b:lbignum len -> i:size_nat{i <= len} -> lbign
 let bn_div_pow2 #len b i =
   slice b i len
 
+
 val bn_div_pow2_lemma: #len:size_nat -> b:lbignum len -> i:size_nat{i < len} ->
   Lemma (bn_v (bn_div_pow2 b i) == bn_v b / pow2 (64 * i))
 let bn_div_pow2_lemma #len c i =
@@ -180,6 +199,9 @@ let bn_mod_pow2_lemma #aLen a i =
     bn_v (slice a 0 i);
     }
 
+///
+///  Conditional swap
+///
 
 //the same as in curve25519
 val lemma_cswap2_step:
@@ -234,19 +256,15 @@ let cswap2 #len bit b1 b2 =
   Loops.repeati len (cswap2_f #len mask) (b1, b2)
 
 
-val cswap2_lemma_:
+val cswap2_lemma:
     #len:size_nat
   -> bit:uint64{v bit <= 1}
   -> b1:lseq uint64 len
   -> b2:lseq uint64 len ->
-  Pure (tuple2 (lseq uint64 len) (lseq uint64 len))
-  (requires True)
-  (ensures fun (p1, p2) ->
-   (let mask = u64 0 -. bit in
-    (p1, p2) == Loops.repeati len (cswap2_f #len mask) (b1, b2) /\
-    (if v bit = 1 then p1 == b2 /\ p2 == b1 else p1 == b1 /\ p2 == b2)))
+  Lemma (let (p1, p2) = cswap2 bit b1 b2 in
+    (if v bit = 1 then p1 == b2 /\ p2 == b1 else p1 == b1 /\ p2 == b2))
 
-let cswap2_lemma_ #len bit b1 b2 =
+let cswap2_lemma #len bit b1 b2 =
   let mask = u64 0 -. bit in
   Loops.eq_repeati0 len (cswap2_f #len mask) (b1, b2);
   let (p1, p2) =
@@ -265,17 +283,387 @@ let cswap2_lemma_ #len bit b1 b2 =
   assert (if v bit = 1 then (eq_intro p2 b1; p2 == b1) else (eq_intro p2 b2; p2 == b2));
   //eq_intro p1 (if v bit = 1 then b2 else b1);
   //eq_intro p2 (if v bit = 1 then b1 else b2);
-  (p1, p2)
-
-
-val cswap2_lemma:
-    #len:size_nat
-  -> bit:uint64{v bit <= 1}
-  -> b1:lseq uint64 len
-  -> b2:lseq uint64 len ->
-  Lemma (let (p1, p2) = cswap2 bit b1 b2 in
-    (if v bit = 1 then p1 == b2 /\ p2 == b1 else p1 == b1 /\ p2 == b2))
-
-let cswap2_lemma #len bit b1 b2 =
-  let _ = cswap2_lemma_ #len bit b1 b2 in
   ()
+
+///
+///  bn_get_num_bits
+///
+
+let bn_leading_zero_index_t (len:size_nat) (i:nat{i <= len}) = x:nat{x < len}
+
+val bn_leading_zero_index_f:
+    #len:size_nat
+  -> b:lbignum len
+  -> i:nat{i < len}
+  -> priv:bn_leading_zero_index_t len i ->
+  bn_leading_zero_index_t len (i + 1)
+
+let bn_leading_zero_index_f #len b i priv =
+  let mask = eq_mask b.[i] (zeros U64 SEC) in
+  if v mask = 0 then i else priv
+
+val bn_leading_zero_index: #len:size_pos -> b:lbignum len -> res:size_nat{res < len}
+let bn_leading_zero_index #len b =
+  Loops.repeat_gen len (bn_leading_zero_index_t len) (bn_leading_zero_index_f #len b) 0
+
+
+val bn_leading_zero_index_lemma: #len:size_pos -> b:lbignum len ->
+  Lemma (let ind = bn_leading_zero_index #len b in
+    ind < len /\ (ind > 0 ==> v b.[ind] <> 0) /\ (forall (k:nat{ind < k /\ k < len}). v b.[k] = 0))
+
+let bn_leading_zero_index_lemma #len b =
+  Loops.eq_repeat_gen0 len (bn_leading_zero_index_t len) (bn_leading_zero_index_f #len b) 0;
+  let res =
+  Loops.repeati_inductive #size_nat len
+  (fun i priv ->
+    priv == Loops.repeat_gen i (bn_leading_zero_index_t len) (bn_leading_zero_index_f #len b) 0 /\
+    priv < len /\ (priv > 0 ==> v b.[priv] <> 0) /\ (forall (k:nat{priv < k /\ k < i}). v b.[k] = 0))
+  (fun i priv ->
+    Loops.unfold_repeat_gen (i + 1) (bn_leading_zero_index_t len) (bn_leading_zero_index_f #len b) 0 i;
+    let mask = eq_mask b.[i] (zeros U64 SEC) in
+    eq_mask_lemma b.[i] (zeros U64 SEC);
+    assert (if v mask = 0 then v b.[i] <> 0 else v b.[i] = 0);
+    let res = if v mask = 0 then i else priv in
+    res) 0 in
+  ()
+
+
+val bn_leading_zero_index_eval_lemma: #len:size_pos -> b:lbignum len -> ind:nat -> Lemma
+  (requires
+    ind < len /\ (ind > 0 ==> v b.[ind] <> 0) /\ (forall (k:nat{ind < k /\ k < len}). v b.[k] = 0))
+  (ensures
+    bn_v b == bn_v (slice b 0 ind) + pow2 (64 * ind) * v b.[ind])
+
+let bn_leading_zero_index_eval_lemma #len b ind =
+  assert (forall (k:nat{ind < k /\ k < len}). v b.[k] = 0);
+  bn_eval_split_i b (ind + 1);
+  assert (bn_v b == bn_v (slice b 0 (ind + 1)) + pow2 (64 * (ind + 1)) * bn_v (slice b (ind + 1) len));
+  eq_intro (slice b (ind + 1) len) (create (len - ind - 1) (u64 0));
+  bn_eval_zeroes (len - ind - 1) (len - ind - 1);
+  assert (bn_v b == bn_v (slice b 0 (ind + 1)));
+  //Seq.slice_slice b 0 (ind + 1) 0 ind;
+  //assert (slice (slice b 0 (ind + 1)) 0 ind == slice b 0 ind);
+  bn_eval_split_i (slice b 0 (ind + 1)) ind;
+  assert (bn_v b == bn_v (slice b 0 ind) + pow2 (64 * ind) * bn_v (slice b ind (ind + 1)));
+  bn_eval1 (slice b ind (ind + 1));
+  assert (bn_v b == bn_v (slice b 0 ind) + pow2 (64 * ind) * v b.[ind])
+
+
+
+let limb_leading_zero_index_t (i:nat{i <= 64}) = x:size_nat{x < 64}
+
+val limb_leading_zero_index_f: a:uint64 -> i:nat{i < 64} -> priv:limb_leading_zero_index_t i -> limb_leading_zero_index_t (i + 1)
+let limb_leading_zero_index_f a i priv =
+  if v (limb_get_ith_bit a i) = 1 then i else priv
+
+
+val limb_leading_zero_index: a:uint64 -> res:size_nat{res < 64}
+let limb_leading_zero_index a =
+  Loops.repeat_gen 64 limb_leading_zero_index_t (limb_leading_zero_index_f a) 0
+
+
+val limb_leading_zero_index_lemma: a:uint64 ->
+  Lemma (let ind = limb_leading_zero_index a in
+    ind < 64 /\ (ind > 0 ==> v (limb_get_ith_bit a ind) = 1) /\
+    (forall (k:nat{ind < k /\ k < 64}). v (limb_get_ith_bit a k) = 0))
+
+let limb_leading_zero_index_lemma a =
+  Loops.eq_repeat_gen0 64 limb_leading_zero_index_t (limb_leading_zero_index_f a) 0;
+  let res =
+  Loops.repeati_inductive #size_nat 64
+  (fun i priv ->
+    priv == Loops.repeat_gen i limb_leading_zero_index_t (limb_leading_zero_index_f a) 0 /\
+    priv < 64 /\ (priv > 0 ==> v (limb_get_ith_bit a priv) = 1) /\
+    (forall (k:nat{priv < k /\ k < i}). v (limb_get_ith_bit a k) = 0))
+  (fun i priv ->
+    Loops.unfold_repeat_gen (i + 1) limb_leading_zero_index_t (limb_leading_zero_index_f a) 0 i;
+    limb_get_ith_bit_lemma a i;
+    let res = if v (limb_get_ith_bit a i) = 1 then i else priv in
+    res) 0 in
+  ()
+
+
+val limb_leading_zero_eval_lemma_aux: a:uint64 -> ind:nat{ind < 64} -> j:nat{ind < j /\ j <= 64} -> Lemma
+  (requires (forall (k:nat{ind < k /\ k < 64}). v a / pow2 k % 2 = 0))
+  (ensures  v a / pow2 j = 0)
+  (decreases (64 - j))
+
+let rec limb_leading_zero_eval_lemma_aux a ind j =
+  if j = 64 then ()
+  else begin
+    limb_leading_zero_eval_lemma_aux a ind (j + 1);
+    assert (v a / pow2 (j + 1) = 0);
+    calc (==) {
+      v a / pow2 j;
+      (==) { Math.Lemmas.euclidean_division_definition (v a / pow2 j) 2 }
+      (v a / pow2 j) / 2 * 2 + v a / pow2 j % 2;
+      (==) { assert_norm (pow2 1 = 2); Math.Lemmas.division_multiplication_lemma (v a) (pow2 j) (pow2 1) }
+      (v a / (pow2 j * pow2 1)) * 2 + v a / pow2 j % 2;
+      (==) { Math.Lemmas.pow2_plus j 1 }
+      (v a / pow2 (j + 1)) * 2 + v a / pow2 j % 2;
+      (==) { }
+      0;
+      }; () end
+
+
+val limb_leading_zero_index_eval_lemma: a:uint64{v a > 0} -> ind:nat -> Lemma
+  (requires
+    ind < 64 /\ (ind > 0 ==> v (limb_get_ith_bit a ind) = 1) /\
+    (forall (k:nat{ind < k /\ k < 64}). v (limb_get_ith_bit a k) = 0))
+  (ensures
+    pow2 ind <= v a /\ v a < pow2 (ind + 1))
+
+let limb_leading_zero_index_eval_lemma a ind =
+  let aux (k:nat{ind < k /\ k < 64}) : Lemma (v a / pow2 k % 2 = 0) =
+    assert (v (limb_get_ith_bit a k) = 0);
+    limb_get_ith_bit_lemma a k;
+    assert (v a / pow2 k % 2 = 0);
+    () in
+  Classical.forall_intro aux;
+  assert (forall (k:nat{ind < k /\ k < 64}). v a / pow2 k % 2 = 0);
+
+  limb_leading_zero_eval_lemma_aux a ind (ind + 1);
+  assert (v a / pow2 (ind + 1) = 0);
+
+  if ind = 0 then begin
+    assert_norm (pow2 0 = 1);
+    assert_norm (pow2 1 = 2);
+    assert (v a = 1) end
+  else begin
+    calc (==) {
+      v a / pow2 ind;
+      (==) { Math.Lemmas.euclidean_division_definition (v a / pow2 ind) 2 }
+      (v a / pow2 ind) / 2 * 2 + v a / pow2 ind % 2;
+      (==) { assert_norm (pow2 1 = 2);
+	Math.Lemmas.division_multiplication_lemma (v a) (pow2 ind) (pow2 1) }
+      (v a / (pow2 ind * pow2 1)) * 2 + v a / pow2 ind % 2;
+      (==) { Math.Lemmas.pow2_plus ind 1 }
+      (v a / pow2 (ind + 1)) * 2 + v a / pow2 ind % 2;
+      (==) { }
+      v a / pow2 ind % 2;
+      (==) { limb_get_ith_bit_lemma a ind }
+      v (limb_get_ith_bit a ind);
+      (==) { }
+      1;
+      };
+    assert (v a / pow2 ind = 1) end;
+
+  calc (==) {
+    v a;
+    (==) { Math.Lemmas.euclidean_division_definition (v a) (pow2 (ind + 1)) }
+    v a % pow2 (ind + 1) + v a / pow2 (ind + 1) * pow2 (ind + 1);
+    (==) { }
+    v a % pow2 (ind + 1);
+    };
+  assert (v a < pow2 (ind + 1));
+
+  calc (==) {
+    v a;
+    (==) { Math.Lemmas.euclidean_division_definition (v a) (pow2 ind) }
+    v a % pow2 ind + v a / pow2 ind * pow2 ind;
+    (==) { }
+    v a % pow2 ind + pow2 ind;
+    };
+  assert (pow2 ind <= v a)
+
+
+val bn_get_num_bits: #len:size_pos{64 * len <= max_size_t} -> b:lbignum len -> size_nat
+let bn_get_num_bits #len b =
+  let ind = bn_leading_zero_index #len b in
+  let bits = limb_leading_zero_index b.[ind] in
+  64 * ind + bits
+
+
+val bn_get_num_bits_lemma_aux: ind:size_nat -> bits:size_nat -> a:nat -> b:nat -> Lemma
+  (requires
+    pow2 bits <= b /\ b < pow2 (bits + 1) /\ a < pow2 (64 * ind))
+  (ensures
+    pow2 (64 * ind + bits) <= a + pow2 (64 * ind) * b /\
+    a + pow2 (64 * ind) * b < pow2 (64 * ind + bits + 1))
+
+let bn_get_num_bits_lemma_aux ind bits a b =
+  calc (>=) {
+    a + pow2 (64 * ind) * b;
+    (>=) { }
+    pow2 (64 * ind) * b;
+    (>=) { }
+    pow2 (64 * ind) * pow2 bits;
+    (==) { Math.Lemmas.pow2_plus (64 * ind) bits }
+    pow2 (64 * ind + bits);
+  };
+  assert (pow2 (64 * ind + bits) <= a + pow2 (64 * ind) * b);
+
+  calc (<=) {
+    a + pow2 (64 * ind) * b;
+    (<=) { }
+    pow2 (64 * ind) - 1 + pow2 (64 * ind) * b;
+    (<=) { }
+    pow2 (64 * ind) - 1 + pow2 (64 * ind) * (pow2 (bits + 1) - 1);
+    (==) { Math.Lemmas.distributivity_sub_right (pow2 (64 * ind)) (pow2 (bits + 1)) 1 }
+    pow2 (64 * ind) * pow2 (bits + 1) - 1;
+    (==) { Math.Lemmas.pow2_plus (64 * ind) (bits + 1) }
+    pow2 (64 * ind + bits + 1) - 1;
+    };
+  assert (a + pow2 (64 * ind) * b < pow2 (64 * ind + bits + 1))
+
+
+val bn_get_num_bits_lemma: #len:size_pos{64 * len <= max_size_t} -> b:lbignum len -> Lemma
+  (requires 0 < bn_v b)
+  (ensures (let bits = bn_get_num_bits b in
+    bits <= 64 * len /\ blocks (bits + 1) 64 <= len /\
+    pow2 bits <= bn_v b /\ bn_v b < pow2 (bits + 1)))
+
+let bn_get_num_bits_lemma #len b =
+  let ind = bn_leading_zero_index #len b in
+  bn_leading_zero_index_lemma b;
+  bn_leading_zero_index_eval_lemma b ind;
+  assert (bn_v b == bn_v (slice b 0 ind) + pow2 (64 * ind) * v b.[ind]);
+  let bits = limb_leading_zero_index b.[ind] in
+  if ind = 0 then begin
+    bn_eval0 (slice b 0 ind);
+    assert_norm (pow2 0 = 1);
+    assert (bn_v b == v b.[ind]);
+    assert (v b.[ind] > 0);
+    () end;
+  assert (v b.[ind] > 0);
+  limb_leading_zero_index_lemma b.[ind];
+  limb_leading_zero_index_eval_lemma b.[ind] bits;
+  assert (pow2 bits <= v b.[ind] /\ v b.[ind] < pow2 (bits + 1));
+
+  bn_eval_bound (slice b 0 ind) ind;
+  bn_get_num_bits_lemma_aux ind bits (bn_v (slice b 0 ind)) (v b.[ind])
+
+
+// val limb_get_num_bits_f: i:nat{i < 6} -> tuple2 uint64 pos -> tuple2 uint64 pos
+// let limb_get_num_bits_f i (l, bits) =
+//   assert_norm (pow2 5 = 32);
+//   Math.Lemmas.pow2_le_compat 5 (5 - i);
+//   let half_t = pow2 (5 - i) in
+//   let x = l >>. size half_t in
+//   let mask = u64 0 -. x in
+//   let mask = u64 0 -. (mask >>. 63ul) in
+//   let bits = if v mask = 0 then bits else bits + half_t in
+//   let l = l ^. (mask &. (x ^. l)) in
+//   (l, bits)
+
+
+// val limb_get_num_bits: a:uint64 -> pos
+// let limb_get_num_bits a =
+//   let (l, bits) = Loops.repeati 6 limb_get_num_bits_f (a, 1) in
+//   bits
+
+// val limb_get_num_bits_f_lemma: i:nat{i < 6} -> lb:tuple2 uint64 pos -> Lemma
+//   (requires (let l, bits = lb in 0 < v l))
+//   (ensures  (let l, bits = lb in
+//     let l1, bits1 = limb_get_num_bits_f i (l, bits) in
+//     let half_t = pow2 (5 - i) in
+//     let x = v l / pow2 half_t in 0 < v l1 /\ 0 < bits1 /\
+//     (if x = 0 then l1 == l /\ bits1 == bits else v l1 == x /\ bits1 == bits + half_t)))
+
+// let limb_get_num_bits_f_lemma i (l, bits) =
+//   let l1, bits1 = limb_get_num_bits_f i (l, bits) in
+//   assert_norm (pow2 5 = 32);
+//   Math.Lemmas.pow2_le_compat 5 (5 - i);
+//   let half_t = pow2 (5 - i) in
+//   let x = l >>. size half_t in
+//   assert (v x == v l / pow2 half_t);
+//   let mask = u64 0 -. x in
+//   if v x = 0 then begin
+//     assert (v mask = 0);
+//     let mask = u64 0 -. (mask >>. 63ul) in
+//     assert (v mask = 0);
+//     assert (bits1 = bits);
+//     BB.mask_select_lemma1 mask x l;
+//     assert (v l1 == v l);
+//     () end
+//   else begin
+//     // assert (v mask == pow2 64 - v x);
+//     assert (v mask == (- v x) % pow2 64);
+//     let mask1 = u64 0 -. (mask >>. 63ul) in
+//     assert (v mask1 = (- v mask / pow2 63) % pow2 64);
+//     calc (==) {
+//       (- v mask / pow2 63) % pow2 64;
+//       (==) { Math.Lemmas.lemma_mod_sub_1 (v mask / pow2 63) (pow2 64) }
+//       pow2 64 - (v mask / pow2 63) % pow2 64;
+//       (==) { Math.Lemmas.modulo_division_lemma (v mask) (pow2 63) (pow2 64) }
+//       pow2 64 - (v mask % (pow2 64 * pow2 63)) / pow2 63;
+//       (==) { Math.Lemmas.pow2_plus 64 63; Math.Lemmas.small_mod (v mask) (pow2 127) }
+//       pow2 64 - v mask / pow2 63;
+//       (==) { }
+//       pow2 64 - 1;
+//       };
+//     assert (v mask1 = v (ones U64 SEC));
+//     assert (bits1 = bits + half_t);
+//     BB.mask_select_lemma1 mask1 x l;
+//     assert (v l1 == v x);
+//     () end
+
+
+// val limb_get_num_bits_lemma_step: l1:pos -> i:pos{i <= 6} -> bits1:pos -> Lemma
+//   (let half_t = pow2 (6 - i) in
+//    let x = l1 / pow2 half_t in
+//    x * pow2 (bits1 + half_t - 1) <= l1 * pow2 (bits1 - 1))
+
+// let limb_get_num_bits_lemma_step l1 i bits1 =
+//   let half_t = pow2 (6 - i) in
+//   let x = l1 / pow2 half_t in
+
+//   calc (>=) {
+//     l1 * pow2 (bits1 - 1);
+//     (>=) { Math.Lemmas.multiply_fractions l1 (pow2 half_t) }
+//     x * pow2 half_t * pow2 (bits1 - 1);
+//     (==) { Math.Lemmas.paren_mul_right x (pow2 half_t) (pow2 (bits1 - 1));
+//       Math.Lemmas.pow2_plus half_t (bits1 - 1) }
+//     x * pow2 (bits1 + half_t - 1);
+//   }
+
+
+// val limb_get_num_bits_lemma_loop: a:uint64{0 < v a} -> i:nat{i <= 6} -> Lemma
+//   (let (l, bits) = Loops.repeati i limb_get_num_bits_f (a, 1) in
+//    let half_t = pow2 (6 - i) in
+//    v l < pow2 half_t /\ 0 < v l /\
+//    v l * pow2 (bits - 1) <= v a)
+
+// let rec limb_get_num_bits_lemma_loop a i =
+//   let (l, bits) = Loops.repeati i limb_get_num_bits_f (a, 1) in
+//   if i = 0 then begin
+//     Loops.eq_repeati0 i limb_get_num_bits_f (a, 1);
+//     assert_norm (pow2 0 = 1);
+//     assert_norm (pow2 1 = 2);
+//     assert_norm (pow2 6 = 64);
+//     () end
+//   else begin
+//     let (l1, bits1) = Loops.repeati (i - 1) limb_get_num_bits_f (a, 1) in
+//     Loops.unfold_repeati i limb_get_num_bits_f (a, 1) (i - 1);
+//     assert ((l, bits) == limb_get_num_bits_f (i - 1) (l1, bits1));
+//     limb_get_num_bits_lemma_loop a (i - 1);
+//     assert (v l1 * pow2 (bits1 - 1) <= v a /\ v l1 < pow2 (pow2 (7 - i)) /\ 0 < v l1 /\ 0 < bits1);
+//     limb_get_num_bits_f_lemma (i - 1) (l1, bits1);
+//     let half_t = pow2 (6 - i) in
+//     let x = v l1 / pow2 half_t in
+//     assert (if x = 0 then l == l1 /\ bits == bits1 else v l == x /\ bits == bits1 + half_t);
+//     assert (v l1 == x * pow2 half_t + v l1 % pow2 half_t);
+
+//     if x = 0 then ()
+//     else begin
+//       assert (pow2 (bits - 1) == pow2 (bits1 + half_t - 1));
+//       Math.Lemmas.pow2_double_sum (6 - i);
+//       Math.Lemmas.lemma_div_lt_nat (v l1) (pow2 (7 - i)) (pow2 (6 - i));
+//       assert (v l < pow2 half_t);
+//       limb_get_num_bits_lemma_step (v l1) i bits1;
+//       assert (v l * pow2 (bits1 + half_t - 1) <= v a);
+//     () end;
+
+//     () end
+
+
+// val limb_get_num_bits_lemma: a:uint64{v a > 0} -> Lemma (pow2 (limb_get_num_bits a - 1) <= v a)
+// let limb_get_num_bits_lemma a =
+//   let bits = limb_get_num_bits a in
+//   assert_norm (pow2 0 = 1);
+//   assert_norm (pow2 1 = 2);
+//   let (l, bits) = Loops.repeati 6 limb_get_num_bits_f (a, 1) in
+//   limb_get_num_bits_lemma_loop a 6;
+//   assert (0 < v l /\ v l < 2);
+//   assert (v l * pow2 (bits - 1) <= v a);
+//   assert (v l = 1)
