code/bignum/Hacl.Spec.Bignum.Exponentiation.fsti
@@ -65,7 +65,6 @@ val bn_mod_exp_mont_ladder_precompr2_lemma:
 // This function is *NOT* constant-time on the exponent b
 val bn_mod_exp:
     nLen:size_pos{128 * nLen <= max_size_t}
-  -> nBits:size_pos
   -> n:lbignum nLen
   -> a:lbignum nLen
   -> bBits:size_pos
@@ -75,7 +74,6 @@ val bn_mod_exp:
 
 val bn_mod_exp_lemma:
     nLen:size_pos{128 * nLen <= max_size_t}
-  -> nBits:size_pos
   -> n:lbignum nLen
   -> a:lbignum nLen
   -> bBits:size_pos
@@ -84,13 +82,12 @@ val bn_mod_exp_lemma:
     bn_v n % 2 = 1 /\ 1 < bn_v n /\ bn_v n < pow2 (64 * nLen) /\
     0 < bn_v b /\ bn_v b < pow2 bBits /\ bn_v a < bn_v n)
   (ensures
-    bn_v (bn_mod_exp nLen nBits n a bBits b) == Lib.NatMod.pow_mod #(bn_v n) (bn_v a) (bn_v b))
+    bn_v (bn_mod_exp nLen n a bBits b) == Lib.NatMod.pow_mod #(bn_v n) (bn_v a) (bn_v b))
 
 
 // This function is constant-time on the exponent b
 val bn_mod_exp_mont_ladder:
     nLen:size_pos{128 * nLen <= max_size_t}
-  -> nBits:size_pos
   -> n:lbignum nLen
   -> a:lbignum nLen
   -> bBits:size_pos
@@ -100,7 +97,6 @@ val bn_mod_exp_mont_ladder:
 
 val bn_mod_exp_mont_ladder_lemma:
     nLen:size_pos{128 * nLen <= max_size_t}
-  -> nBits:size_pos
   -> n:lbignum nLen
   -> a:lbignum nLen
   -> bBits:size_pos
@@ -109,4 +105,4 @@ val bn_mod_exp_mont_ladder_lemma:
     bn_v n % 2 = 1 /\ 1 < bn_v n /\ bn_v n < pow2 (64 * nLen) /\
     0 < bn_v b /\ bn_v b < pow2 bBits /\ bn_v a < bn_v n)
   (ensures
-    bn_v (bn_mod_exp_mont_ladder nLen nBits n a bBits b) == Lib.NatMod.pow_mod #(bn_v n) (bn_v a) (bn_v b))
+    bn_v (bn_mod_exp_mont_ladder nLen n a bBits b) == Lib.NatMod.pow_mod #(bn_v n) (bn_v a) (bn_v b))
